\documentclass[12pt]{article}

% Packages
\usepackage{amsmath}	% eqn *
\usepackage{amssymb}	% mathbb
\usepackage{amsthm}
\usepackage{units}

% Margin Setup
\usepackage[paperwidth=8.5in, paperheight=11.0in,
left=1.5in, right=1.0in, top=1.0in,
bottom=1.0in, includefoot, heightrounded]{geometry}

% Custom Commands
\newcommand{\tByt}[9]{
	\left[\begin{array}{c c c}
		#1 & #2 & #3 \\
		#4 & #5 & #6 \\
		#7 & #8 & #9 \\
		\end{array}\right]
}
\newcommand{\tvec}[3]
{	
	\left[
	\begin{array}{c}
		#1 \\ #2 \\ #3
	\end{array}
	\right]
}
\newcommand{\dx}{\Delta x}

\begin{document}

\section{General Expansions}
\begin{align*}
f(x+\dx) &= f(x)+f'(x)\dx + \frac{1}{2}f''(x)\dx^2+\frac{1}{6}f'''(x)\dx^3+O(\dx^4)\\
f(x-\dx) &= f(x)-f'(x)\dx + \frac{1}{2}f''(x)\dx^2-\frac{1}{6}f'''(x)\dx^3+O(\dx^4)\\
f(x+2\dx) &= f(x)+2f'(x)\dx + 2f''(x)\dx^2+\frac{4}{3}f'''(x)\dx^3+O(\dx^4) \\
f(x-2\dx) &= f(x)-2f'(x)\dx + 2f''(x)\dx^2-\frac{4}{3}f'''(x)\dx^3+O(\dx^4) \\
f(x+3\dx) &= f(x)+3f'(x)\dx + \frac{9}{2}f''(x)\dx^2+\frac{9}{2}f'''(x)\dx^3+O(\dx^4) \\
f(x-3\dx) &= f(x)-3f'(x)\dx + \frac{9}{2}f''(x)\dx^2-\frac{9}{2}f'''(x)\dx^3+O(\dx^4) \\
\end{align*}
\section{Second-Order Differences}
\subsection{Centered Difference}
\begin{align*}
f_{i+1}-f_{i-1} = 2f'(x)\dx+O(\dx^3) &\rightarrow f'(x) = \frac{f_{i+1}-f_{i-1}}{2\dx} + O(\dx^2) \\
f_{i+1}+f_{i-1} = 2f(x)+f''(x)\dx^2+O(\dx^4) &\rightarrow f''(x) = \frac{f_{i+1}-2f_i+f_{i-1}}{\dx^2} + O(\dx^2) 
\end{align*}
\subsection{Forward Difference}
\newcommand{\del}{\Delta}
\begin{align*}
\del_1 &= f_{i+1}-f_{i} = f'(x)\dx + \frac{1}{2}f''(x)\dx^2+\frac{1}{6}f'''(x)\dx^3+O(\dx^4)\\
\del_2 &= f_{i+2}-f_{i} = 2f'(x)\dx + 2f''(x)\dx^2+\frac{4}{3}f'''(x)\dx^3+O(\dx^4) \\
\del_3 &= f_{i+3}-f_{i} = 3f'(x)\dx + \frac{9}{2}f''(x)\dx^2+\frac{9}{2}f'''(x)\dx^3+O(\dx^4)
\end{align*}
\begin{equation*}
\tByt{1}{\nicefrac{1}{2}}{\nicefrac{1}{6}}{2}{2}{\nicefrac{4}{3}}{3}{\nicefrac{9}{2}}{\nicefrac{9}{2}}\tvec{f'(x)\dx}{f''(x)\dx^2}{f'''(x)\dx^3} = \tvec{\del_1}{\del_2}{\del_3} + O(\dx^4)
\end{equation*}
\begin{equation*}
\tvec{f'(x)}{f''(x)}{f'''(x)}= \tvec{(3\del_1-\frac{3}{2}\del_2+\frac{1}{3}\del_3)/(\dx)}{(-5\del_1+4\del_2-\del_3)/(\dx^2)}{(3\del_1-3\del_2+\del_3)/(\dx^3)}+\tvec{O(\dx^3)}{O(\dx^2)}{O(\dx)}
\end{equation*}
\subsection{Backward Difference}
\begin{align*}
\del_1 &= f_{i}-f_{i-1} = -f'(x)\dx + \frac{1}{2}f''(x)\dx^2-\frac{1}{6}f'''(x)\dx^3+O(\dx^4)\\
\del_2 &= f_{i}-f_{i-2} = -2f'(x)\dx + 2f''(x)\dx^2-\frac{4}{3}f'''(x)\dx^3+O(\dx^4) \\
\del_3 &= f_{i}-f_{i-3} = -3f'(x)\dx + \frac{9}{2}f''(x)\dx^2-\frac{9}{2}f'''(x)\dx^3+O(\dx^4)
\end{align*}
\begin{equation*}
\tByt{-1}{\nicefrac{1}{2}}{-\nicefrac{1}{6}}{-2}{2}{-\nicefrac{4}{3}}{-3}{\nicefrac{9}{2}}{-\nicefrac{9}{2}}\tvec{f'(x)\dx}{f''(x)\dx^2}{f'''(x)\dx^3} = \tvec{\del_1}{\del_2}{\del_3} + O(\dx^4)
\end{equation*}
\begin{equation*}
\tvec{f'(x)}{f''(x)}{f'''(x)}= \tvec{(-3\del_1+\frac{3}{2}\del_2-\frac{1}{3}\del_3)/(\dx)}{(-5\del_1+4\del_2-\del_3)/(\dx^2)}{(-3\del_1+3\del_2-\del_3)/(\dx^3)}+\tvec{O(\dx^3)}{O(\dx^2)}{O(\dx)}
\end{equation*}
\end{document}